src/Disks/CowZonedDisk.dfy
@@ -1,0 +1,199 @@
+/* A terrible but "straightforward" block-addressible translation layer: All
+ * zones are of a fixed size, and (n-1) zones are available for user use, with
+ * one reserved as a buffer.  A random access write to a particular zone
+ * necessitates a full copy of that zone to the buffer zone, applying the
+ * destructive update in place.
+ *
+ * When the final block is written to the disk, a zone map is updated in order
+ * to make the copy "durable".
+ *
+ * Yeah, this sucks!  Nobody should build a drive this way, but the intention
+ * here is to get a trivial remapping system working and show refinement, before
+ * we show something more interesting.
+ */
+
+include "../Types.dfy"
+include "../Disk.dfy"
+include "../Utils.dfy"
+
+include "ZonedDisk.dfy"
+
+module CowZonedDisk refines Disk {
+    import opened NativeTypes
+    import opened Types
+    import opened Utils
+
+    import Block
+    import Zone
+    import ZonedDisk
+
+    datatype Constants = Constants(
+        zd: ZonedDisk.Constants
+    )
+
+    datatype State = State(
+        /* The underlying zoned disk */
+        zd: ZonedDisk.State,
+
+        /* Which buffer will we fault the next write's zone over into? */
+        buffer_zone: int,
+
+        /* Logical zone -> physical zone remapping (to account for the
+         * buffer zone, which will float around as writes happen) */
+        buffer_map: seq<int>
+    )
+
+    function method Init(c: Constants) : State
+    {
+        State(
+            ZonedDisk.Init(c.zd),
+
+            /* Begin with the identity mapping for the first (n-1) zones,
+             * leaving the final zone for our initial buffer.  */
+            c.zd.n_blocks as int - 1,
+            seq(c.zd.n_blocks - 1, i => i)
+        )
+    }
+
+    predicate ConstantsValid(c: Constants)
+    {
+        && ZonedDisk.ConstantsValid(c.zd)
+        && forall i,j :: 0 <= i < j < |c.zd.zone_map| ==> 
+            c.zd.zone_map[i].1 - c.zd.zone_map[i].0 
+            == c.zd.zone_map[j].1 - c.zd.zone_map[j].0
+
+    }
+
+    predicate Valid(c: Constants, s: State)
+    {
+        && ZonedDisk.Valid(c.zd, s.zd)
+        && 0 <= s.buffer_zone as int < |s.zd.zones|
+        && buffer_map_well_formed(c, s)
+    }
+
+    predicate lba_in_range(c: Constants, lba: uint64)
+        requires ConstantsValid(c)
+    {
+        c.zd.zone_map[0].0 <= lba < c.zd.zone_map[|c.zd.zone_map| - 1].1
+    }
+
+    predicate buffer_map_well_formed(c: Constants, s: State)
+    {
+        var map_max := |c.zd.zone_map| - 1;
+        var bmap := s.buffer_map;
+
+        // the buffer map needs to be a permutation of [0..|c.zd.zone_map|)
+        // with exactly one element missing, namely buffer_zone.
+        && |s.buffer_map| == |c.zd.zone_map| - 1
+        && forall i :: 0 <= i       < |bmap| ==> 0 <= bmap[i] <= map_max
+        && forall i,j :: 0 <= i < j < |bmap| ==> bmap[i] != bmap[j]
+        && forall i :: 0 <= i       < |bmap| ==> bmap[i] != s.buffer_zone
+
+        // The buffer zone needs to be in range, and it has to be empty.
+        && 0 <= s.buffer_zone < |s.zd.zones|
+        && Zone.Empty(s.zd.zones[s.buffer_zone])
+    }
+
+    function Read(c: Constants, s: State, lba: uint64) : Block.State
+        requires Valid(c, s)
+        ensures Block.Valid(Read(c, s, lba))
+    {
+        var p :| ZonedDisk.resolve_lba(c.zd, lba, p);
+        var (lzone, off) := p;
+        var pzone := s.buffer_map[lzone];
+
+        s.zd.zones[pzone].blocks[off]
+    }
+
+    // XXX: This will do a full zone copy.  Where should the fact that this involves
+    // multiple atomic operaitons live?  That could be at the refinement layer, but
+    // maybe it needs to be here?
+    predicate Write(c: Constants, s: State, s': State, lba: uint64, val: Block.State)
+        requires Valid(c, s)
+    {
+        var p :| ZonedDisk.resolve_lba(c.zd, lba, p);
+        var (lzone, off) := p;
+        var pzone := s.buffer_map[lzone];
+
+        var src_zone := s.zd.zones[pzone];
+        var dst_zone := Zone.State(
+            MaxUInt64(src_zone.write_ptr + 1, off) as uint64,
+            src_zone.blocks[ off := val ]
+        );
+
+        assert Zone.Valid(dst_zone);
+
+        && |s.zd.zones| == |s'.zd.zones|
+
+        // The zone containing the block we want to destructively write
+        // is now the new buffer zone
+        && Zone.Empty(s'.zd.zones[pzone])
+
+        // Our former buffer zone now contains the zone with the
+        // destructive update
+        && Zone.Empty(s.zd.zones[s.buffer_zone])
+        && s'.zd.zones[s.buffer_zone] == dst_zone
+
+        // No other zones are touched
+        && forall i :: 0 <= i < |s'.zd.zones| ==>
+            (&& i != pzone 
+            && i != s.buffer_zone ==> s.zd.zones[i] == s'.zd.zones[i])
+    }
+
+
+    // Steps and step relations
+
+    datatype Step =
+    | ReadBlock(lba: uint64, val: Block.State)
+    | WriteBlock(lba: uint64, val: Block.State)
+
+    predicate NextStep(c: Constants, s: State, s': State, step: Step)
+    {
+        Valid(c, s) 
+        && match step {
+            case ReadBlock(off, val) => 
+                && lba_in_range(c, off) ==>
+                && Read(c, s, off) == val
+            case WriteBlock(off, val) => 
+                && lba_in_range(c, off) ==>
+                && Write(c, s, s', off, val)
+        }       
+    }
+
+    predicate Next(c: Constants, s: State, s': State)
+    {
+        exists step :: NextStep(c, s, s', step)
+    }
+
+    // Invariant preservation
+    
+    lemma InitImpliesValid(c: Constants) 
+    {}
+
+    lemma NextPreservesValid(c: Constants, s: State, s': State)
+        requires Valid(c, s)
+        requires Next(c, s, s')
+        ensures Valid(c, s')
+    {
+        var step :| NextStep(c, s, s', step);
+        match step {
+            case ReadBlock(off, val) => ReadPreservesValid(c, s, s', off, val);
+            case WriteBlock(off, val) => WritePreservesValid(c, s, s', off, val);
+        }
+    }
+
+    lemma ReadPreservesValid(c: Constants, s: State, s': State, lba: uint64, val: Block.State)
+        requires Valid(c, s)
+        requires lba_in_range(c, lba)
+        requires s == s'
+        requires Read(c, s, lba) == val
+        ensures Valid(c, s')
+    {}
+    
+    lemma WritePreservesValid(c: Constants, s: State, s': State, lba: uint64, val: Block.State)
+        requires Valid(c, s)
+        requires Write(c, s, s', lba, val);
+        ensures Valid(c, s')
+    {}
+
+}
