src/Utils.dfy
@@ -1,0 +1,17 @@
+include "Types.dfy"
+
+module Utils {
+    import opened NativeTypes
+
+    // what's polymorphism, precious?
+
+    function method MinUInt64(a: uint64, b: uint64): uint64
+    {
+        if a < b then a else b
+    }
+
+    function method MaxUInt64(a: uint64, b: uint64): uint64
+    {
+        if a > b then a else b
+    }
+}
